paper/WIP/proof/check_kernel.v
@@ -2,3 +2,5 @@ Require Import Kernel.
 Print Assumptions kernel_correct.
 Print Assumptions kernel_first_spec.
 Print Assumptions goal_reachable_correct.
+Print Assumptions goal_reach_implies_reach_mu.
+Print Assumptions goal_reach_strictly_stronger.
